lakefile.lean
@@ -51,8 +51,8 @@ lean_lib «Contracts» where
     .andSubmodules `Contracts.ReentrancyRelyGuarantee
   ]
 
-lean_lib «SoliditySliceSmoke» where
-  globs := #[.one `Contracts.SoliditySliceSmoke.Smoke]
+lean_lib «SolidityImportSmoke» where
+  globs := #[.one `Contracts.SolidityImportSmoke.Smoke]
 
 lean_lib «Compiler» where
   globs := #[.andSubmodules `Compiler]
